AwsCryptographicMaterialProviders/dafny/AwsCryptographyKeyStore/src/KMSKeystoreOperations.dfy
@@ -642,6 +642,8 @@ module {:options "/functionSyntax:4" } KMSKeystoreOperations {
   )
     returns (output: Result<KMS.DecryptResponse, Types.Error>)
 
+    requires HvUtils.HasUniqueTransformedKeys?(encryptionContextToKms)
+
     requires kmsClient.ValidState()
     modifies kmsClient.Modifies
     ensures kmsClient.ValidState()
